Backup tex document

doc/coq/Equiv.v
@@ -2,7 +2,7 @@ From MODULAR Require Export Sound.
 
 Generalizable Variables T TT.
 
-Definition equiv_st `{time T} `{time TT} (f : T -> TT)
+Definition equiv_st `{OrderT T} `{OrderT TT} (f : T -> TT)
   (st : @state T) (st' : @state TT) :=
   match st, st' with
   | ST mem t, ST mem' t' =>
@@ -16,34 +16,48 @@ Definition equiv_st `{time T} `{time TT} (f : T -> TT)
       end
   end.
 
+Definition in_dom {T} (t : T) (C : @dy_ctx T) (st : @state T) :=
+  match st with
+  | ST mem t' => t = t' \/ In_ctx t C \/ mem t <> None
+  end.
+
+Definition inc_on_dom `{OT : OrderT T} `{OTT : OrderT TT} (f : T -> TT) (C : @dy_ctx T) (st : @state T) :=
+  forall (t t' : T) (INt : in_dom t C st) (INt' : in_dom t' C st),
+    t < t' -> f t < f t'.
+
 Lemma equiv_eval : 
   forall `{time T} `{time TT} 
          (C : @dy_ctx T) st e v st_v
-         (EVAL : EvalR C st e v st_v)
          (BOUND : time_bound C st)
+         (EVAL : EvalR C st e v st_v)
          (C' : @dy_ctx TT) st' f
+         (BOUND' : time_bound C' st')
+         (INC : inc_on_dom f C st)
          (EQC : trans_ctx f C = C')
          (EQS : equiv_st f st st'),
     exists C_v' st_v' f',
       match st with
       | ST _ t =>
         eq_bound t f f' /\
+        time_bound C_v' st_v' /\
         match v with
         | EVal (Closure x e_v C_v) =>
+          inc_on_dom f' C_v st_v /\
           trans_ctx f' C_v = C_v' /\
           equiv_st f' st_v st_v' /\
           EvalR C' st' e (EVal (Closure x e_v C_v')) st_v'
         | MVal C_v =>
+          inc_on_dom f' C_v st_v /\
           trans_ctx f' C_v = C_v' /\
           equiv_st f' st_v st_v' /\
           EvalR C' st' e (MVal C_v') st_v'
         end
       end.
 Proof.
-  intros. 
+  intros.
   rename H into ET. rename H0 into OT. rename H1 into tT.
   rename H2 into ETT. rename H3 into OTT. rename H4 into tTT.
-  revert BOUND C' st' f EQC EQS.
+  revert C' st' f BOUND' INC EQC EQS.
   induction EVAL; intros; simpl in *.
   - rewrite <- STATE in EQS.
     simpl in EQS. destruct st' as [mem' t'].
@@ -53,13 +67,24 @@ Proof.
     destruct (mem' (f addr)) eqn:ACCESS'; try inversion EQS'.
     destruct e as [x'' e_v' C_v'].
     exists C_v'. exists (ST mem' t'). exists f.
-    rewrite <- STATE. repeat split; try assumption.
+    unfold inc_on_dom in INC. rewrite <- STATE in *.
+    repeat split; try assumption.
+    destruct EQS' as [? [? RR]]. rewrite <- RR.
+    rewrite eqb_eq in H. rewrite <- H.
+    assert (dy_ctx_bound C_v t).
+    { destruct BOUND as [? [? ?]].
+      pose proof (p_bound_or_not addr t) as cases.
+      destruct cases as [CASE | CASE].
+      specialize (H4 addr CASE). rewrite <- ACCESS in H4. eauto.
+      specialize (H3 addr CASE). rewrite <- ACCESS in H3. inversion H3. }
+    apply INC; eauto. apply INC; eauto.
     apply EQS'. 
     apply Eval_var_e with (addr := f addr) (mem := mem') (t := t'); eauto.
     rewrite <- EQC. rewrite trans_ctx_addr. rewrite <- ADDR. eauto.
     rewrite ACCESS'. destruct EQS' as [EQx [EQe EQc]]. subst; eauto.
   - exists C'. exists st'. exists f.
-    destruct st. repeat split; eauto.
+    unfold inc_on_dom in *. destruct st. repeat split; try assumption.
+    apply INC; eauto. apply INC; eauto. eauto.
   - pose proof (time_bound_e C st e1 (EVal (Closure x e C_lam)) st_lam EVAL1) as BOUND'.
     pose proof (time_bound_e C st_lam e2 (EVal arg) (ST mem t) EVAL2) as BOUND''.
     pose proof (time_bound_e (C_lam [|dy_c_lam x t ([||])|])
@@ -109,21 +134,80 @@ Proof.
       try apply relax_ctx_bound with (t1 := t); try apply update_lt. eauto. inversion BB2''. }
     specialize (BOUND''' B2).
     specialize (IHEVAL1 BOUND). specialize (IHEVAL2 B1). specialize (IHEVAL3 B2).
-    specialize (IHEVAL1 C' st' f EQC EQS).
-    destruct IHEVAL1 as [C_v' [st_v' [f' [BB [EQClam [EQstlam EVALlam]]]]]].
+    specialize (IHEVAL1 C' st' f INC EQC EQS).
+    destruct IHEVAL1 as [C_v' [st_v' [f' [BB [INClam [EQClam [EQstlam EVALlam]]]]]]].
     assert (trans_ctx f' C = C') as EQC'.
     { rewrite <- EQC. symmetry. 
       apply bound_trans_ctx_eq with (t := t0); eauto. apply BOUND. }
-    specialize (IHEVAL2 C' st_v' f' EQC' EQstlam). 
-    destruct IHEVAL2 as [C_v'' [st_v'' [f'' [BB' [EQCarg [EQstarg EVALarg]]]]]].
+    specialize (IHEVAL2 C' st_v' f' INClam EQC' EQstlam). 
+    destruct IHEVAL2 as [C_v'' [st_v'' [f'' [BB' [INCarg [EQCarg [EQstarg EVALarg]]]]]]].
     assert (trans_ctx f'' (C_lam [|dy_c_lam x t ([||])|]) = (C_v' [|dy_c_lam x (f'' t) ([||])|])) as EQC''.
     { rewrite plugin_trans_ctx. simpl.
       rewrite <- EQClam.
       assert (trans_ctx f' C_lam = trans_ctx f'' C_lam) as RR.
       apply bound_trans_ctx_eq with (t := t1); eauto. apply BOUND'.
       rewrite RR. eauto. }
+    destruct st_v'' as [mem'' t''].
     remember (fun t' => if eqb t' (update C (ST mem t) x (Closure x0 e0 C0))
-                        then Abs.update abs_C (Abs.ST mem'' t'') x (Closure x0 e0 abs_C'') 
-                        else α'' t') as α'''.
-    specialize (IHEVAL3 (C_v' [|dy_c_lam x (f'' t) ([||])|]) st_v'' f'' EQC'' EQstarg).
+                        then update C' (ST mem'' t'') x (Closure x0 e0 C_v'') 
+                        else f'' t') as f'''.
+    assert (eq_bound t f'' f''') as BB''.
+    { red. intros. rewrite Heqf'''. 
+      assert (eqb t' (update C (ST mem t) x (Closure x0 e0 C0)) = false) as RR.
+      refl_bool. intros contra. rewrite eqb_eq in contra.
+      assert (leb t t' = true). rewrite contra. apply update_lt. 
+      assert (t = t') as RR. apply leb_sym; eauto. rewrite <- RR in contra.
+      clear RR.
+      assert (eqb t (update C (ST mem t) x (Closure x0 e0 C0)) <> true).
+      refl_bool. apply update_lt. apply H0. rewrite <- contra. apply eqb_refl.
+      rewrite RR. eauto. }
+    assert (equiv_st f''' 
+            (ST (t !-> Closure x0 e0 C0; mem)
+                (update C (ST mem t) x (Closure x0 e0 C0)))
+            (ST ((f'' t) !-> Closure x0 e0 C_v''; mem'')
+                (update C' (ST mem'' t'') x (Closure x0 e0 C_v'')))).
+    { simpl. split.
+      - rewrite Heqf'''. rewrite eqb_refl. apply eqb_eq. eauto.
+      - intros. unfold update_m.
+        destruct (eqb addr t) eqn:ADDR.
+        + rewrite eqb_eq in ADDR. rewrite ADDR.
+          rewrite Heqf'''. rewrite eqb_update. rewrite eqb_refl; repeat split; eauto.
+          rewrite <- EQCarg. symmetry. apply bound_trans_ctx_eq with (t := t).
+          apply BOUND''. rewrite EQCarg. rewrite <- Heqf'''. apply BB''.
+        + pose proof (p_bound_or_not addr t) as CASES.
+          destruct BOUND'' as [B1'' [B2'' B3'']].
+          destruct CASES as [L | R]; 
+          try (specialize (B3'' addr L); try rewrite B3''; eauto);
+          try (specialize (B2'' addr R); try rewrite B2''; eauto).
+          assert (f''' addr = f'' addr) as RR. symmetry. apply BB''. apply L. rewrite RR; clear RR.
+          destruct EQstarg as [? H].
+          specialize (H addr) as HINT.
+          destruct (mem addr) eqn: ACCESS'; eauto. 
+          destruct e4; simpl.
+          assert (f'' addr < f'' t) as RR.
+          { apply INCarg; eauto.
+            red. left. red. intros contra. rewrite ACCESS' in contra. inversion contra.
+            red. right. eauto. }
+          destruct RR as [RR RR']. rewrite RR'. clear RR RR'.
+          assert (trans_ctx f'' C2 = trans_ctx f''' C2) as RR.
+          { apply bound_trans_ctx_eq with (t := t); eauto. } rewrite <- RR; clear RR. eauto.
+          destruct (eqb (f'' addr) (f'' t)) eqn:EQ; eauto.
+          rewrite eqb_eq in EQ. rewrite EQ in HINT.
+          destruct (mem t). destruct e5. rewrite  rewrite ACCESS in HINT'. rewrite ACCESS' in HINT.
+          simpl. right. symmetry in Heqb0. rewrite eqb_eq in Heqb0.
+          rewrite <- Heqb0. apply HINT; eauto. apply HINT; eauto.
+    }
+    {rewrite plugin_trans_ctx; simpl. rewrite Heqα'''.
+        rewrite eqb_update. rewrite <- Heqα'''.
+        assert (trans_ctx α''' C_lam = abs_C'). rewrite Heqα'''.
+        destruct abs_st'. simpl in SOUND'. destruct SOUND' as [[? [? ?]] ?]. rewrite <- H0.
+        apply bound_trans_ctx_eq with (t := t1). apply BOUND'.
+        red. intros. assert (eqb t' (update C (ST mem t) x (Closure x0 e0 C0)) = false).
+        refl_bool. intros contra. rewrite eqb_eq in contra.
+        assert (leb t' t = true). lebt t1.
+        assert (t = t') as RR. apply leb_sym; try assumption. rewrite contra. apply update_lt.
+        assert (t < t') as contra'. rewrite contra. apply update_lt.
+        destruct contra' as [? contra']. rewrite RR in contra'. rewrite eqb_refl in contra'. inversion contra'.
+        rewrite H3. symmetry. apply EQ''. assumption. rewrite H. eauto.}
+    specialize (IHEVAL3 (C_v' [|dy_c_lam x (f'' t) ([||])|]) (ST mem'' t'') f'' EQC'' EQstarg).
 
